Revise FunMaps.v

FunMaps.v
@@ -1,6 +1,8 @@
 Require Import
   Here.FMapExt
   Here.Nomega
+  Coq.Sets.Ensembles
+  Here.TupleEnsembles
   Coq.FSets.FMapList
   Coq.FSets.FMapFacts
   Coq.Structures.OrderedTypeEx.
@@ -10,57 +12,55 @@ Module FunMaps (O : OrderedType).
 Module E := FMapExt(O).
 Include E.
 
-Program Definition to_rel {A} (m : M.t A) : FunRel M.key A :=
-  M.fold (fun k e r => Insert k e r _) m (Empty M.key A).
-Obligation 1.
-Admitted.
-
-Definition SetMap_AbsR {A B}
-           (or : FunRel M.key A) (nr : M.t B)
-           (AbsR : A -> B -> Prop) : Prop :=
+Definition SetMap_AbsR
+           (A B : Type) (R  : A -> B -> Prop)
+           (or : Ensemble (M.key * A))
+           (nr : M.t B) : Prop :=
   forall addr,
     (forall blk,
        Lookup addr blk or
-         -> (exists cblk, M.find addr nr = Some cblk /\ AbsR blk cblk)) /\
+         -> (exists cblk, M.find addr nr = Some cblk /\ R blk cblk)) /\
     (forall cblk,
        M.find addr nr = Some cblk
-         -> (exists blk, Lookup addr blk or /\ AbsR blk cblk)).
-
-Lemma Empty_SetMap_AbsR : forall A B R,
-  SetMap_AbsR (Empty M.key A) (M.empty B) R.
-Proof.
-  split; intros.
-    inversion H.
-  apply F.find_mapsto_iff, F.empty_mapsto_iff in H.
-  contradiction.
-Qed.
+         -> (exists blk, Lookup addr blk or /\ R blk cblk)).
 
 Ltac reduction :=
-  teardown; subst;
-  try match goal with
+  try repeat teardown; subst;
+  match goal with
+  | [ _ : ?T -> ?U -> Prop,
+      H1 : SetMap_AbsR _ _ _,
+      H2 : Lookup ?A ?D ?K |- exists _ : ?U, _ ] =>
+    let HA := fresh "HA" in
+    destruct (H1 A) as [HA _];
+    let HC := fresh "HC" in
+    let HD := fresh "HC" in
+    let cblk := fresh "cblk" in
+    destruct (HA _ H2) as [cblk [HC HD]]; clear HA H2;
+    exists cblk; split; trivial
   | [ H1 : SetMap_AbsR _ _ _,
       H2 : Lookup ?A ?D ?K |- _ ] =>
     let HA := fresh "HA" in
     let HB := fresh "HB" in
-    destruct (H1 A) as [HA HB]; clear H1;
+    destruct (H1 A) as [HA HB];
     let HC := fresh "HC" in
     let HD := fresh "HD" in
     let cblk := fresh "cblk" in
     destruct (HA _ H2) as [cblk [HC HD]]; clear HA HB H2
-  | [ H1 : SetMap_AbsR _ _ _,
-      H2 : In _ (relEns ?K) (?A, ?D) |- _ ] =>
-    let HA := fresh "HA" in
+  | [ _ : ?T -> ?U -> Prop,
+      H1 : SetMap_AbsR _ _ _,
+      H2 : M.find ?A ?K = Some ?D |- exists _ : ?T, _ ] =>
     let HB := fresh "HB" in
-    destruct (H1 A) as [HA HB]; clear H1;
+    destruct (H1 A) as [_ HB];
     let HC := fresh "HC" in
     let HD := fresh "HD" in
-    let cblk := fresh "cblk" in
-    destruct (HA _ H2) as [cblk [HC HD]]; clear HA HB H2
+    let blk := fresh "blk" in
+    destruct (HB _ H2) as [blk [HC HD]]; clear HB H2;
+    exists blk; split; trivial
   | [ H1 : SetMap_AbsR _ _ _,
       H2 : M.find ?A ?K = Some ?D |- _ ] =>
     let HA := fresh "HA" in
     let HB := fresh "HB" in
-    destruct (H1 A) as [HA HB]; clear H1;
+    destruct (H1 A) as [HA HB];
     let HC := fresh "HC" in
     let HD := fresh "HD" in
     let blk := fresh "blk" in
@@ -71,89 +71,76 @@ Section FunMaps_AbsR.
 
 Variables A B : Type.
 Variable R  : A -> B -> Prop.
-Variable or : FunRel M.key A.
+Variable or : Ensemble (M.key * A).
 Variable nr : M.t B.
-Variable H  : SetMap_AbsR or nr R.
+Variable AbsR : SetMap_AbsR R or nr.
 
-Lemma SetMap_AbsR_prj1 : forall (addr : M.key) (blk : A) cblk,
-  Ensembles.In _ (relEns or) (addr, blk)
+Lemma Empty_SetMap_AbsR : SetMap_AbsR R Empty (M.empty B).
+Proof.
+  split; intros.
+    inversion H.
+  apply F.find_mapsto_iff, F.empty_mapsto_iff in H.
+  contradiction.
+Qed.
+
+Corollary SetMap_AbsR_prj1 : forall (addr : M.key) (blk : A) cblk,
+  Lookup addr blk or
     -> (forall a b c, R a b -> R a c -> b = c)
     -> R blk cblk
     -> M.find (elt:=B) addr nr = Some cblk.
-Proof.
-  intros.
-  destruct (H addr); clear H.
-  destruct (H3 _ H0) as [cblk' [? ?]]; clear H0 H3.
-  rewrite (H1 _ _ _ H2 H5); assumption.
-Qed.
+Proof. intros; reduction; rewrite (H0 _ _ _ H1 HD); assumption. Qed.
 
-Lemma SetMap_AbsR_prj1_ex : forall (addr : M.key) (blk : A),
-  Ensembles.In _ (relEns or) (addr, blk)
+Corollary SetMap_AbsR_prj1_ex : forall (addr : M.key) (blk : A),
+  Lookup addr blk or
     -> exists cblk : B,
          M.find (elt:=B) addr nr = Some cblk /\ R blk cblk.
-Proof.
-  intros.
-  destruct (H addr); clear H.
-  destruct (H1 _ H0) as [cblk [? ?]]; clear H0 H1.
-  exists cblk; auto.
-Qed.
+Proof. intros; reduction. Qed.
 
-Lemma SetMap_AbsR_prj2_ex : forall (addr : M.key) (cblk : B),
+Corollary SetMap_AbsR_prj2_ex : forall (addr : M.key) (cblk : B),
   M.find (elt:=B) addr nr = Some cblk
     -> exists blk : A, Lookup addr blk or /\ R blk cblk.
-Proof.
-  intros.
-  destruct (H addr); clear H.
-  destruct (H2 _ H0) as [blk [? ?]]; clear H0 H2.
-  exists blk; auto.
-Qed.
+Proof. intros. reduction. Qed.
 
 Hypothesis Oeq_eq : forall a b, O.eq a b -> a = b.
 
 Lemma Update_SetMap_AbsR : forall k v v',
-  R v v' -> SetMap_AbsR (Update k v or) (M.add k v' nr) R.
+  R v v' -> SetMap_AbsR R (Update k v or) (M.add k v' nr).
 Proof.
   split; intros.
-    reduction.
-      exists v'.
-      split; trivial.
+  - repeat teardown; subst.
+    + exists v'; split; trivial.
       apply F.find_mapsto_iff, F.add_mapsto_iff.
       left; auto.
-    exists cblk.
-    intuition.
-    apply F.find_mapsto_iff in HC.
-    apply F.find_mapsto_iff, F.add_mapsto_iff.
-    right; split; auto.
-  apply F.find_mapsto_iff, F.add_mapsto_iff in H1.
-  destruct H1; destruct H1; subst.
-    exists v.
-    split; trivial.
-    apply Oeq_eq in H1; subst.
-    right; constructor.
-  apply F.find_mapsto_iff in H2.
-  reduction; exists blk.
-  intuition.
-  left; constructor; auto.
-  unfold Ensembles.In; simpl.
-  unfold not; intros.
-  subst; auto.
+    + reduction.
+      apply F.find_mapsto_iff in HC.
+      apply F.find_mapsto_iff, F.add_mapsto_iff.
+      right; split; auto.
+  - apply F.find_mapsto_iff, F.add_mapsto_iff in H0.
+    destruct H0, H0; subst.
+      exists v; split; trivial.
+      apply Oeq_eq in H0; subst.
+      right; constructor.
+    apply F.find_mapsto_iff in H1.
+    reduction.
+    left; constructor; auto.
+    unfold Ensembles.In; simpl.
+    unfold not; intros.
+    subst; auto.
 Qed.
 
 Lemma Remove_SetMap_AbsR : forall k,
-  SetMap_AbsR (Remove k or) (M.remove k nr) R.
+  SetMap_AbsR R (Remove k or) (M.remove k nr).
 Proof.
   split; intros.
-    reduction; exists cblk.
-    intuition.
+    reduction.
     apply F.find_mapsto_iff, F.remove_mapsto_iff.
     split; auto.
     apply F.find_mapsto_iff.
     assumption.
-  apply F.find_mapsto_iff, F.remove_mapsto_iff in H0.
-  destruct H0.
-  apply F.find_mapsto_iff in H1.
-  reduction; exists blk.
-  intuition.
+  apply F.find_mapsto_iff, F.remove_mapsto_iff in H.
+  destruct H.
+  apply F.find_mapsto_iff in H0.
+  reduction.
   constructor; trivial.
   unfold Ensembles.In; simpl.
   unfold not; intros.
@@ -161,37 +148,37 @@ Proof.
 Qed.
 
 Lemma Map_SetMap_AbsR : forall f f',
-  (forall i a b, R a b -> R (f (i, a)) (f' i b))
-    -> SetMap_AbsR (Map f or) (M.mapi f' nr) R.
+  (forall i a b, R a b -> R (f i a) (f' i b))
+    -> SetMap_AbsR R (Map f or) (M.mapi f' nr).
 Proof.
   split; intros.
-    teardown; subst.
-    destruct (H addr); clear H H3.
-    destruct (H1 _ H2) as [cblk [? ?]]; clear H1 H2.
-    apply F.find_mapsto_iff in H.
+    repeat teardown; subst.
+    destruct (AbsR addr); clear H2.
+    destruct (H0 _ H1) as [cblk [? ?]]; clear H0 H1.
     exists (f' addr cblk).
+    apply F.find_mapsto_iff in H2.
     split.
       rewrite F.mapi_o, <- F.map_o.
         apply F.find_mapsto_iff.
         apply F.map_mapsto_iff.
         exists cblk; tauto.
       intros.
-      apply Oeq_eq in H1.
+      apply Oeq_eq in H0.
       subst; reflexivity.
-    apply H0; trivial.
-  rewrite F.mapi_o, <- F.map_o in H1.
+    apply H; trivial.
+  rewrite F.mapi_o, <- F.map_o in H0.
+    apply F.find_mapsto_iff in H0.
+    apply F.map_mapsto_iff in H0.
+    repeat teardown; subst.
     apply F.find_mapsto_iff in H1.
-    apply F.map_mapsto_iff in H1.
-    destruct H1; destruct H1; subst.
-    apply F.find_mapsto_iff in H2.
-    destruct (H addr); clear H H1.
-    destruct (H3 _ H2) as [blk [? ?]]; clear H2 H3.
-    exists (f (addr, blk)).
+    destruct (AbsR addr); clear H0.
+    destruct (H2 _ H1) as [blk [? ?]]; clear H1 H2.
+    exists (f addr blk).
     split.
-      apply Lookup_Map; trivial.
-    apply H0; trivial.
+      teardown.
+    apply H; trivial.
   intros.
-  apply Oeq_eq in H2.
+  apply Oeq_eq in H1.
   subst; reflexivity.
 Qed.
 
@@ -205,123 +192,23 @@ Proof.
   reflexivity.
 Qed.
 
-Lemma Partition_SetMap_AbsR
-      (f : M.key -> A -> Prop)
-      (f' : M.key -> B -> bool)
-      (f'_Proper : Proper (O.eq ==> eq ==> eq) f')  :
-  (forall a b, R a b -> forall i, Bool.reflect (f i a) (f' i b))
-    -> forall a a', Partition f or = (a, a')
-    -> forall b b', P.partition f' nr = (b, b')
-    -> SetMap_AbsR a b R /\ SetMap_AbsR a' b' R.
-Proof.
-  split; intros; split; intros.
-  - unfold Partition in H0.
-    unfold P.partition in H1.
-    inversion H0; subst; clear H0;
-    inversion H1; subst; clear H1;
-    simpl in H2; destruct H2.
-    destruct (H addr) as [H3 _].
-    destruct (H3 _ H1) as [cblk [? ?]]; clear H1 H3.
-    exists cblk; intuition.
-    apply F.find_mapsto_iff.
-    apply F.find_mapsto_iff in H2.
-    apply P.filter_iff; intuition.
-    destruct (X _ _ H4 addr); intuition.
-Admitted.
-(*
-  - destruct (H addr); clear H H1.
-    apply F.find_mapsto_iff in H0.
-    apply P.filter_iff in H0; trivial.
-    destruct H0.
-    apply F.find_mapsto_iff in H.
-    destruct (H2 _ H) as [blk [? ?]]; clear H H2.
-    exists blk; intuition.
-    split; intuition.
-    destruct (X _ _ H3 addr); intuition.
-  - destruct (H addr); clear H H2.
-    destruct H0.
-    destruct (H1 _ H0) as [cblk [? ?]]; clear H0 H1.
-    exists cblk; intuition.
-    apply F.find_mapsto_iff.
-    apply F.find_mapsto_iff in H2.
-    apply P.filter_iff; intuition.
-    apply Proper_Oeq_negb; assumption.
-    apply negb_true_iff.
-    destruct (X _ _ H3 addr); intuition.
-  - destruct (H addr); clear H H1.
-    apply F.find_mapsto_iff in H0.
-    apply P.filter_iff in H0; trivial.
-    destruct H0.
-    apply negb_true_iff in H0.
-    apply F.find_mapsto_iff in H.
-    destruct (H2 _ H) as [blk [? ?]]; clear H H2.
-    exists blk; intuition.
-    split; intuition.
-      destruct (X _ _ H3 addr); intuition.
-    apply Proper_Oeq_negb; assumption.
-Qed.
-*)
-
-Lemma Same_set_SetMap_AbsR : forall a b r HF,
-  Same_set _ (relEns a) b
-    -> SetMap_AbsR a r R
-    -> SetMap_AbsR (mkFunRel b HF) r R.
-Proof.
-  intros.
-  intros addr.
-  destruct (H1 addr); clear H1.
-  split; intros.
-    unfold Lookup in H1.
-    unfold Same_set, Included in H0.
-    destruct H0.
-    apply H4 in H1.
-    destruct (H2 _ H1) as [cblk [? ?]].
-    exists cblk.
-    intuition.
-  destruct (H3 _ H1) as [blk [? ?]].
-  exists blk.
-  unfold Same_set, Included in H0.
-  destruct H0.
-  apply H0 in H4.
-  intuition.
-Qed.
-
-Lemma foo : forall A x y (z : A),
-  (x = Some z <-> y = Some z)
-    -> (x = None <-> y = None)
-    -> x = y.
-Proof.
-Admitted.
-
-Lemma Equal_SetMap_AbsR : forall a b b',
-  SetMap_AbsR a b R
-    -> SetMap_AbsR a b' R
-    -> M.Equal b b'.
-Proof.
-  intros.
-  intro addr.
-  destruct (H0 addr), (H1 addr).
-  destruct (M.find (elt:=B) addr b').
-  apply foo with (z:=b0); split; intros; trivial.
-Abort.
-
 Lemma Single_SetMap_AbsR : forall base blk cblk,
-  R blk cblk -> SetMap_AbsR (Single base blk) (singleton base cblk) R.
+  R blk cblk -> SetMap_AbsR R (Single base blk) (singleton base cblk).
 Proof.
   intros.
   intro addr.
   split; intros;
   [exists cblk|exists blk].
-    inversion H1; subst.
+    repeat teardown; subst.
     split; trivial.
-    unfold singleton.
+    unfold P.uncurry.
     rewrite F.elements_o; simpl.
     rewrite eqb_refl.
     reflexivity.
-  rewrite F.elements_o in H1; simpl in H1.
-  unfold F.eqb in H1.
+  rewrite F.elements_o in H0; simpl in H0.
+  unfold F.eqb in H0.
   destruct (O.eq_dec addr base).
-    inversion H1.
+    inversion H0.
     apply Oeq_eq in e.
     subst.
     split; trivial.
@@ -330,5 +217,43 @@ Proof.
 Qed.
 
 End FunMaps_AbsR.
+
+Lemma Same_set_SetMap_AbsR : forall A B (R : A -> B -> Prop) a b r,
+  Same a b
+    -> SetMap_AbsR R a r
+    -> SetMap_AbsR R b r.
+Proof.
+  intros.
+  intros addr.
+  destruct (H0 addr).
+  split; intros.
+    apply H in H3.
+    destruct (H1 _ H3) as [cblk [? ?]].
+    exists cblk.
+    intuition.
+  destruct (H2 _ H3) as [blk [? ?]].
+  exists blk.
+  split; trivial.
+  apply H; trivial.
+Qed.
+
+Lemma Equal_SetMap_AbsR : forall A B (R : A -> B -> Prop) a b r,
+  M.Equal a b
+    -> SetMap_AbsR R r a
+    -> SetMap_AbsR R r b.
+Proof.
+  intros.
+  intros addr.
+  destruct (H0 addr).
+  split; intros.
+    destruct (H1 _ H3) as [cblk [? ?]].
+    exists cblk.
+    split; trivial.
+    rewrite <- H; trivial.
+  rewrite <- H in H3.
+  destruct (H2 _ H3) as [blk [? ?]].
+  exists blk.
+  intuition.
+Qed.
 
 End FunMaps.
